How do I separation logic?

thy/PointerMapImpl.thy
@@ -5,30 +5,64 @@ imports ArrayList
   PointerMap
 begin
 
-  record 'a pointer_map_impl =
+  record 'a pointermap_impl =
     entriesi :: "'a array_list"
     getentryi :: "('a,nat) hashtable"
 
-  definition is_pointer_map_impl where
-    "is_pointer_map_impl b bi \<equiv> 
+  definition is_pointermap_impl where
+    "is_pointermap_impl b bi \<equiv> 
       is_array_list (entries b) (entriesi bi) 
     * is_hashmap (getentry b) (getentryi bi)"
 
-  lemma "precise is_pointer_map_impl"
-  	unfolding is_pointer_map_impl_def[abs_def]
+  lemma "precise is_pointermap_impl"
+  	unfolding is_pointermap_impl_def[abs_def]
   	apply(rule preciseI)
+  	apply(auto)
   	using preciseD[OF is_array_list_prec] preciseD[OF is_hashmap_prec]
-  	apply- 
+  	unfolding mod_and_dist 
   	find_theorems "_ \<Turnstile> _ * _"
     sorry
 
-  definition init_bdd_impl :: "bdd_impl" where
-    "init_bdd_impl \<equiv> do {
-      
+  definition pointermap_empty where
+    "pointermap_empty \<equiv> do {
+      hm \<leftarrow> hm_new;
+      arl \<leftarrow> arl_empty;
+      return \<lparr>entriesi = arl, getentryi = hm \<rparr>
+    }"
 
+  lemma [sep_heap_rules]: "< emp > pointermap_empty <is_pointermap_impl empty_pointermap>\<^sub>t"
+    by (sep_auto simp: pointermap_empty_def empty_pointermap_def is_pointermap_impl_def)
 
-    }"   
+  definition pm_pthi where
+    "pm_pthi m p \<equiv> arl_nth (entriesi m) p"
 
+  lemma [sep_heap_rules]: "pointermap_p_valid p m \<Longrightarrow> < is_pointermap_impl m mi > pm_pthi mi p <\<lambda>ai. \<up>(ai = pm_pth m p)>\<^sub>t"
+    by (sep_auto simp: pm_pthi_def pm_pth_def is_pointermap_impl_def pointermap_p_valid_def)
 
-
+  definition pointermap_getmki where
+    "pointermap_getmki a m \<equiv> do {
+        lo \<leftarrow> ht_lookup a (getentryi m);
+        (case lo of 
+        	Some l \<Rightarrow> return (l,m) | 
+        	None \<Rightarrow> do {
+        		p \<leftarrow> return (snd (entriesi m));
+				ent \<leftarrow> arl_append (entriesi m) a;
+				lut \<leftarrow> hm_update a p (getentryi m);
+				u \<leftarrow> return \<lparr>entriesi = ent, getentryi = lut\<rparr>;
+				return (p,u)
+        	}
+        )
+    }"
+  lemma [sep_heap_rules]: "(p,u) = pointermap_getmk a m \<Longrightarrow> < is_pointermap_impl m mi > pointermap_getmki a mi <\<lambda>(pi,ui). is_pointermap_impl u ui * \<up>(pi = p)>\<^sub>t"
+  unfolding pointermap_getmki_def pointermap_getmk_def pointermap_insert_def is_pointermap_impl_def
+  	apply (sep_auto simp: pointermap_getmki_def pointermap_getmk_def pointermap_insert_def is_pointermap_impl_def ) 
+  	apply(rename_tac b c d e f) (* no idea what they even are *)
+  	apply(rule_tac x = "(e,f)" in is_array_list_lengthI)
+  	find_theorems "_ \<Turnstile> _ * ?a \<Longrightarrow> _ \<Turnstile> ?a" (* how do I even separate? *)
+    apply (sep_auto simp: pointermap_getmki_def pointermap_getmk_def pointermap_insert_def is_pointermap_impl_def is_array_list_def  intro: is_array_list_lengthI split: prod.splits)
+    defer
+    (* I quit for now *)
+    defer
+    oops
+   
 end
